IMLTT/proofs/BoundaryConditions.lean
@@ -6,33 +6,109 @@ import IMLTT.proofs.admissable.Weakening
 
 /- # Boundary conditions -/
 
-theorem boundary_ctx_term : HasType Γ a A → IsCtx Γ :=
-  sorry
 
-theorem boundary_ctx_term_eq : IsEqualTerm Γ a b A → IsCtx Γ :=
-  sorry
+theorem boundary_ctx_type' : IsType Γ A → IsCtx Γ := sorry
+mutual
+  theorem boundary_ctx_term : HasType Γ a A → IsCtx Γ :=
+    by
+      intro haA
+      match haA with
+      | .var hA =>
+        have hiC := boundary_ctx_type' hA
+        apply IsCtx.extend hiC hA
+      -- | .weak hvA hB =>
+      --   have hiC := boundary_ctx_term hvA
+      --   apply IsCtx.extend hiC hB
+      | .unit_intro hiC => --> base
+        apply hiC
+      | .pi_intro hbB =>
+        have hiCA := boundary_ctx_term hbB
+        match hiCA with
+        | .extend hiC  hA => 
+          apply hiC
+      | .sigma_intro hA hB =>
+        have hiC := boundary_ctx_term hA
+        apply hiC
+      | .iden_intro hA =>
+        have hiC := boundary_ctx_term hA
+        apply hiC
+      | .univ_unit hiC =>
+        apply hiC
+      | .univ_empty hiC =>
+        apply hiC
+      | .univ_pi hAU hBU =>
+        have hiC := boundary_ctx_term hAU
+        apply hiC
+      | .univ_sigma hAU hBU =>
+        have hiC := boundary_ctx_term hAU
+        apply hiC
+      | .univ_iden hAU haA haA' =>
+        have hiC := boundary_ctx_term hAU
+        apply hiC
+      | .unit_elim hA haA hbUn =>
+        have hiC := boundary_ctx_term haA
+        apply hiC
+      | .empty_elim hA hbEm =>
+        have hiC := boundary_ctx_term hbEm
+        apply hiC
+      | .pi_elim hfPi haA =>
+        have hiC := boundary_ctx_term haA
+        apply hiC
+      | .sigma_elim hpSi hC hcC =>
+        have hiC := boundary_ctx_term hpSi
+        apply hiC
+      | .iden_elim hB hbB hpI =>
+        have hiC := boundary_ctx_term hpI
+        apply hiC
+      | .ty_conv haA hAB =>
+        have hiC := boundary_ctx_term haA
+        apply hiC
 
-theorem boundary_ctx_type : IsType Γ A → IsCtx Γ :=
-  by
-    intro hA
-    match hA with
-    | .unit_form hiC =>
-      apply hiC
-    | .empty_form hiC =>
-      apply hiC
-    | .pi_form hA hB =>
-      apply boundary_ctx_type hA
-    | .sigma_form hA hB =>
-      apply boundary_ctx_type hA
-    | .iden_form haA haA' =>
-      apply boundary_ctx_term haA
-    | .univ_form hiC =>
-      apply hiC
-    | .univ_elim hAU =>
-      apply boundary_ctx_term hAU
+  theorem boundary_ctx_type : IsType Γ A → IsCtx Γ :=
+    by
+      intro hA
+      match hA with
+      | .unit_form hiC =>
+        apply hiC
+      | .empty_form hiC =>
+        apply hiC
+      | .pi_form hA hB =>
+        apply boundary_ctx_type hA
+      | .sigma_form hA hB =>
+        apply boundary_ctx_type hA
+      | .iden_form haA haA' =>
+        apply boundary_ctx_term haA
+      | .univ_form hiC =>
+        apply hiC
+      | .univ_elim hAU =>
+        apply boundary_ctx_term hAU
+end
 
-theorem boundary_ctx_type_eq : IsEqualType Γ A B → IsCtx Γ :=
-  sorry
+mutual
+  theorem boundary_ctx_term_eq : IsEqualTerm Γ a b A → IsCtx Γ :=
+    sorry
+
+  theorem boundary_ctx_type_eq : IsEqualType Γ A A → IsCtx Γ :=
+    by
+      intro hAA
+      match hAA with
+      | .unit_form_eq hiC =>
+        apply hiC
+      | .empty_form_eq hiC =>
+        apply hiC
+      | .pi_form_eq hAA' hBB' =>
+        apply boundary_ctx_type_eq hAA'
+      | .sigma_form_eq hAA' hBB' =>
+        apply boundary_ctx_type_eq hAA'
+      | .iden_form_eq haa haa' =>
+        apply boundary_ctx_term_eq haa
+      | .univ_form_eq hiC =>
+        apply hiC
+      | .univ_elim_eq hAAU =>
+        apply boundary_ctx_term_eq hAAU
+end
+
+/- # if hasType, then type is well-formed -/
 
 theorem boundary_term_type : HasType Γ a A → IsType Γ A :=
   sorry
@@ -40,7 +116,8 @@ theorem boundary_term_type : HasType Γ a A → IsType Γ A :=
 theorem boundary_equal_term_type : IsEqualTerm Γ a a' A → IsType Γ A :=
   sorry
 
-/- # Closed term check -/
+/-# if substiution works, then adding type to context also -/
 
-theorem closed_lift_eq : lift l j tm = tm :=
+theorem boundary_subs_type_ctx : IsType Γ (substitute A (.extend σ' b))  → HasType Γ b B
+                                 → IsType (Γ ⬝ B) A :=
   sorry
