IMLTT/proofs/admissable/DefeqRelation.lean
@@ -1,0 +1,265 @@
+import IMLTT.untyped.AbstractSyntax
+import IMLTT.untyped.Weakening
+import IMLTT.untyped.Substitution
+import IMLTT.typed.JudgmentsAndRules
+import IMLTT.proofs.BoundaryConditions
+import IMLTT.proofs.admissable.Contexts
+
+/- # Definitional Equality is Equivalence Relation -/
+
+mutual
+  theorem defeq_term_refl : HasType Γ a A → IsEqualTerm Γ a a A :=
+    by
+      intro haA
+      match haA with
+      | .var hA =>
+        apply IsEqualTerm.var_eq
+        apply hA
+      | .unit_intro hiC =>
+        apply IsEqualTerm.unit_intro_eq hiC
+      | .pi_intro hbB =>
+        apply IsEqualTerm.pi_intro_eq
+        · apply defeq_type_refl
+          have hiCA := boundary_ctx_term hbB
+          match hiCA with
+          | .extend hiC hA =>
+            apply hA
+        · apply defeq_type_refl
+          apply boundary_term_type
+          apply hbB
+        · apply defeq_term_refl
+          apply hbB
+      | .sigma_intro haA' hbB' =>
+        apply IsEqualTerm.sigma_intro_eq
+        · apply defeq_type_refl
+          apply boundary_term_type haA'
+        · apply defeq_type_refl
+          have hBs := boundary_term_type hbB'
+          apply boundary_subs_type_ctx hBs haA'
+        · apply defeq_term_refl
+          apply haA'
+        · apply defeq_term_refl
+          apply hbB'
+      | .iden_intro hA =>
+        apply IsEqualTerm.iden_intro_eq
+        apply defeq_term_refl
+        apply hA
+      -- univ start
+      | .univ_unit hiC =>
+        apply IsEqualTerm.univ_unit_eq hiC
+      | .univ_empty hiC =>
+        apply IsEqualTerm.univ_empty_eq hiC
+      | .univ_pi hAU hBU =>
+        apply IsEqualTerm.univ_pi_eq
+        · apply defeq_term_refl
+          apply hAU
+        · apply defeq_term_refl
+          apply hBU
+      | .univ_sigma hAU hBU =>
+        apply IsEqualTerm.univ_sigma_eq
+        · apply defeq_term_refl
+          apply hAU
+        · apply defeq_term_refl
+          apply hBU
+      | .univ_iden hAU haA haA' =>
+        apply IsEqualTerm.univ_iden_eq
+        · apply defeq_term_refl
+          apply hAU
+        · apply defeq_term_refl
+          apply haA
+        · apply defeq_term_refl
+          apply haA'
+      -- univ end
+      | .unit_elim hA haA hbUn =>
+        apply IsEqualTerm.unit_elim_eq
+        · apply defeq_type_refl
+          apply hA
+        · apply defeq_term_refl
+          apply haA
+        · apply defeq_term_refl
+          apply hbUn
+      | .empty_elim hA hbEm =>
+        apply IsEqualTerm.empty_elim_eq
+        · apply defeq_type_refl
+          apply hA
+        · apply defeq_term_refl
+          apply hbEm
+      | .pi_elim hfPi haA =>
+        apply IsEqualTerm.pi_elim_eq
+        · apply defeq_type_refl
+          apply boundary_term_type hfPi
+        · apply defeq_term_refl
+          apply haA
+        · apply defeq_term_refl
+          apply hfPi
+      | .sigma_elim hpPi hC hcC =>
+        apply IsEqualTerm.sigma_elim_eq
+        · apply defeq_type_refl
+          apply boundary_term_type hpPi
+        · apply defeq_term_refl
+          apply hpPi
+        · apply defeq_type_refl
+          apply hC
+        · apply defeq_term_refl
+          apply hcC
+      | .iden_elim hB hbB hpI =>
+        apply IsEqualTerm.iden_elim_eq
+        · apply defeq_type_refl
+          apply hB
+        · apply defeq_term_refl
+          apply hbB
+        · apply defeq_term_refl
+          apply hpI
+      | .ty_conv haA hAB =>
+        apply IsEqualTerm.ty_conv_eq
+        · apply defeq_term_refl
+          apply haA
+        · apply hAB
+
+  theorem defeq_type_refl : IsType Γ A → IsEqualType Γ A A :=
+    fun hA : IsType Γ A ↦
+      match hA with
+      | .unit_form hiC =>
+        by 
+          apply IsEqualType.unit_form_eq hiC
+      | .empty_form hiC  =>
+        by 
+          apply IsEqualType.empty_form_eq hiC
+      | .pi_form hA hB =>
+        by 
+          apply IsEqualType.pi_form_eq
+          · apply defeq_type_refl hA
+          · apply defeq_type_refl hB
+      | IsType.sigma_form hA hB =>
+        by 
+          apply IsEqualType.sigma_form_eq
+          · apply defeq_type_refl hA
+          · apply defeq_type_refl hB
+      | IsType.iden_form haA haA' =>
+        by 
+          apply IsEqualType.iden_form_eq
+          · apply defeq_term_refl haA
+          · apply defeq_term_refl haA'
+      | IsType.univ_form hiC =>
+        by
+          apply IsEqualType.univ_form_eq hiC
+      | IsType.univ_elim hAU =>
+        by
+          apply IsEqualType.univ_elim_eq
+          apply defeq_term_refl hAU
+end
+
+theorem defeq_term_symm : IsEqualTerm Γ a b A → IsEqualTerm Γ b a A :=
+  by
+    intro habA
+    match habA with
+    | .var_eq hA => sorry
+    | .unit_comp hC hcC => sorry
+    | .pi_comp hbB haA => sorry
+    | .sigma_comp haA hbB hC hcC => sorry
+    | .iden_comp hB hbB haA  => sorry
+    | .unit_intro_eq hiC => sorry
+    | .unit_elim_eq hAA haaA hbbUn => sorry
+    | .empty_elim_eq hAA hbbEm => sorry
+    | .pi_intro_eq hAA hBB hbbB => sorry
+    | .pi_elim_eq hPiPi haaA hffPi => sorry
+    | .sigma_intro_eq hAA hBB haaA hbbB => sorry
+    | .sigma_elim_eq hSiSi hppSi hCC hccC => sorry
+    | .iden_intro_eq hAA  => sorry
+    | .iden_elim_eq hAA hBB hbbB => sorry
+    | .ty_conv_eq habA hAB => sorry
+
+theorem defeq_type_symm : IsEqualType Γ A B → IsEqualType Γ B A :=
+  fun hABet : IsEqualType Γ A B ↦
+    match hABet with
+    | .unit_form_eq hic =>
+      by
+        apply IsEqualType.unit_form_eq hic
+    | .empty_form_eq hic =>
+      by
+        apply IsEqualType.empty_form_eq hic
+    | .pi_form_eq hAA hBB =>
+      by
+        apply IsEqualType.pi_form_eq
+        · apply defeq_type_symm hAA
+        · have hBB' := by apply context_conv_is_equal_type hBB hAA
+          apply defeq_type_symm hBB'
+    | .sigma_form_eq hAA hBB =>
+      by
+        apply IsEqualType.sigma_form_eq
+        · apply defeq_type_symm hAA
+        · have hBB' := by apply context_conv_is_equal_type hBB hAA
+          apply defeq_type_symm hBB'
+    | .iden_form_eq haaA haaA' =>
+      by
+        apply IsEqualType.iden_form_eq
+        · apply defeq_term_symm haaA
+        · apply defeq_term_symm haaA'
+    | .univ_form_eq hic =>
+      by
+        apply IsEqualType.univ_form_eq hic
+    | .univ_elim_eq hAAU =>
+      by
+        apply IsEqualType.univ_elim_eq
+        apply defeq_term_symm
+        apply hAAU
+
+
+theorem defeq_term_trans : IsEqualTerm Γ a b A → IsEqualTerm Γ b c A → IsEqualTerm Γ a c A :=
+  by
+    intro habA hbcA
+    sorry
+    -- match habA with
+    -- | .var_eq hA => sorry
+    -- | .unit_comp hC hcC => sorry
+    -- | .pi_comp hbB haA => sorry
+    -- | .sigma_comp haA hbB hC hcC => sorry
+    -- | .iden_comp hB hbB haA => sorry
+    -- | .unit_intro_eq hiC => sorry
+    -- | .unit_elim_eq hAA haaA hbbUn => sorry
+    -- | .empty_elim_eq hAA hbbEm => sorry
+    -- | .pi_intro_eq hAA hBB hbbB => sorry
+    -- | .pi_elim_eq hPiPi haaA hffPi => sorry
+    -- | .sigma_intro_eq hAA hBB haaA hbbB => sorry
+    -- | .sigma_elim_eq hSiSi hppSi hCC hccC => sorry
+    -- | .iden_intro_eq hAA  => sorry
+    -- | .iden_elim_eq hAA hBB hbbB => sorry
+    -- | .ty_conv_eq habA hAB => sorry
+
+
+theorem defeq_type_trans : IsEqualType Γ A B → IsEqualType Γ B C → IsEqualType Γ A C :=
+  fun hAB : IsEqualType Γ A B ↦
+    fun hBC : IsEqualType Γ B C ↦
+    match hAB with
+    | .unit_form_eq hic =>
+      by 
+        apply hBC
+    | .empty_form_eq hic =>
+      by 
+        apply hBC
+    | .pi_form_eq hAA hBB =>
+      by
+        cases hBC with
+        | pi_form_eq hAAc hBBc =>
+          apply IsEqualType.pi_form_eq
+          · apply defeq_type_trans hAA hAAc
+          · have hBBs := context_conv_is_equal_type hBBc (defeq_type_symm hAA)
+            apply defeq_type_trans hBB hBBs
+        | univ_elim_eq hPiC =>
+          apply IsEqualType.univ_elim_eq
+          have hPiPi := (IsEqualType.pi_form_eq hAA hBB)
+          sorry -- apply defeq_term_trans hPiPi hPiC 
+       --  sorry -- TODO: stuck? looping here -> use term transitivity
+       --                                     -> inversions lemma (C gleich Pi), dann rausziehen
+    | .sigma_form_eq hAA hBB =>
+      by 
+        sorry    
+    | .iden_form_eq haaA haaA' =>
+      by 
+        sorry
+    | .univ_form_eq hic => 
+      by 
+        apply hBC
+    | .univ_elim_eq hAAU =>
+      by 
+        sorry
