IMLTT/proofs/admissable/Substitution.lean
@@ -1,27 +1,28 @@
-import IMLTT.AbstractSyntax
-import IMLTT.Substitution
-import IMLTT.JudgmentsAndRules
+import IMLTT.untyped.AbstractSyntax
+import IMLTT.untyped.Substitution
+import IMLTT.typed.JudgmentsAndRules
 
 /- # Substitution Property -/
 
 theorem substitution_ctx : HasType Γ a A → IsCtx (Γ ⬝ A ⬝ B)
-                           → IsCtx (Γ ⬝ (substitute B a 0)) :=
+                           → IsCtx (Γ ⬝ (substitute_zero B a)) :=
   sorry
 
 theorem substitution_type : HasType Γ a A → IsType (Γ ⬝ A) B 
-                            → IsType Γ (substitute B a 0) :=
+                            → IsType Γ (substitute_zero B a) :=
   sorry
 
 theorem substitution_term : HasType Γ a A → HasType (Γ ⬝ A) b B
-                            → HasType Γ (substitute b A 0) (substitute B A 0) :=
+                            → HasType Γ (substitute_zero b A) (substitute_zero B A) :=
   sorry
 
 theorem substitution_type_eq : HasType Γ a A → IsEqualType (Γ ⬝ A) B B'
-                               → IsEqualType Γ (substitute B a 0) (substitute B' a 0) :=
+                               → IsEqualType Γ (substitute_zero B a) (substitute_zero B' a) :=
   sorry
 
 theorem substitution_term_eq : HasType Γ a A → IsEqualTerm (Γ ⬝ A) b b' B
-                               → IsEqualTerm Γ (substitute b a 0) (substitute b' a 0) (substitute B a 0) :=
+                               → IsEqualTerm Γ (substitute_zero b a) (substitute_zero b' a) 
+                                 (substitute_zero B a) :=
   sorry
 
 /- # Substitution inverse -/
@@ -30,78 +31,63 @@ theorem nat_not_less_than_zero : ¬ (i < 0) :=
   by
     apply Nat.not_succ_le_zero
 
-theorem substitution_var_eq_inverse :
-    Tm.var (n - 2) = (substitute (substitute (Tm.var n) (Tm.var 0) 0) (Tm.var 0) 0) :=
-  by
-    induction n with
-    | zero =>
-      simp [substitute]
-    | succ n' ihj =>
-      simp [substitute]
-      simp [nat_not_less_than_zero]
-      cases n' with
-      | zero =>
-        simp [lift]
-      | succ n'' =>
-        simp []
+-- theorem substitution_eq_inverse : A = weaken (substitute_zero (substitute_zero A (.var 0)) (.var 0)) 
+--                                       (.shift (.shift .id)) :=
+--   by
+--     induction A with
+--     | unit =>
+--       simp [substitute]
+--     | pi A B ihA ihB =>
+--       simp [substitute]
+--       simp [lift]
+--       apply And.intro
+--       · apply ihA
+--       sorry
+--     | var n => sorry
+--     | _ => sorry
 
--- FIXME: not doable with current meta operations
-theorem substitution_eq_inverse : A = (substitute (substitute A (Tm.var 0) 0) 0 0) :=
-  by
-    induction A with
-    | unit =>
-      simp [substitute]
-    | pi A B ihA ihB =>
-      simp [substitute]
-      simp [lift]
-      apply And.intro
-      · apply ihA
-      sorry
-    | var n => sorry
-    | _ => sorry
+-- theorem substitute_type_eq_inverse : IsEqualType Γ A A' 
+--                                      = IsEqualType Γ (substitute (substitute A (.var i) j) j i)
+--                                        (substitute (substitute A' i j) j i) :=
+--   by
+--     sorry
 
-theorem substitute_type_eq_inverse : IsEqualType Γ A A' 
-                                     = IsEqualType Γ (substitute (substitute A (Tm.var i) j) j i)
-                                       (substitute (substitute A' i j) j i) :=
-  by
-    sorry
-
-theorem substitution_id_lift : (substitute A (Tm.var i) i) = A := -- FIXME: -1?
-  by
-    sorry
-  --   induction A generalizing i with
-  --   | unit =>
-  --     rw [substitute]
-  --     rw [lift]
-  --   | empty =>
-  --     rw [substitute]
-  --     rw [lift]
-  --   | pi A B ihA ihB =>
-  --     rw [substitute]
-  --     rw [lift]
-  --     rw [ihA]
-  --     rw [←ihB]
-  --     rw [lift]
-  --     simp [nat_not_less_than_zero]
-  --   | sigma A B ihA ihB =>
-  --     rw [substitute]
-  --     rw [lift]
-  --     rw [ihA]
-  --     rw [←ihB]
-  --     rw [lift]
-  --     simp [nat_not_less_than_zero]
-  --   | var n =>
-  --     rw [substitute]
-  --     cases i with
-  --     | zero => 
-  --       simp [nat_not_less_than_zero]
-  --       cases n with
-  --       | zero =>
-  --         simp []
-  --         simp [lift]
-  --       | succ n' =>
-  --         simp []
-  --         simp [lift]
-  --     | succ i' =>
-  --       sorry
-  --   | _ => sorry
+-- theorem substitution_id_lift : (substitute A (Tm.var i) i) = A :=
+--   by
+--     sorry
+--   --   induction A generalizing i with
+--   --   | unit =>
+--   --     rw [substitute]
+--   --     rw [lift]
+--   --   | empty =>
+--   --     rw [substitute]
+--   --     rw [lift]
+--   --   | pi A B ihA ihB =>
+--   --     rw [substitute]
+--   --     rw [lift]
+--   --     rw [ihA]
+--   --     rw [←ihB]
+--   --     rw [lift]
+--   --     simp [nat_not_less_than_zero]
+--   --   | sigma A B ihA ihB =>
+--   --     rw [substitute]
+--   --     rw [lift]
+--   --     rw [ihA]
+--   --     rw [←ihB]
+--   --     rw [lift]
+--   --     simp [nat_not_less_than_zero]
+--   --   | var n =>
+--   --     rw [substitute]
+--   --     cases i with
+--   --     | zero => 
+--   --       simp [nat_not_less_than_zero]
+--   --       cases n with
+--   --       | zero =>
+--   --         simp []
+--   --         simp [lift]
+--   --       | succ n' =>
+--   --         simp []
+--   --         simp [lift]
+--   --     | succ i' =>
+--   --       sorry
+--   --   | _ => sorry
