IMLTT/proofs/admissable/Weakening.lean
@@ -6,28 +6,36 @@ import IMLTT.typed.JudgmentsAndRules
 /- # Weakening -/
 
 theorem weakening_ctx : IsCtx (Γ ⬝ A) → IsType Γ B
-                        → IsCtx (Γ ⬝ B ⬝ (lift 0 1 A)) :=
+                        → IsCtx (Γ ⬝ B ⬝ (weaken A (.shift .id))) :=
   by
     sorry
 
 theorem weakening_type : IsType Γ A → IsType Γ B
-                         → IsType (Γ ⬝ B) (lift 0 1 A) :=
+                         → IsType (Γ ⬝ B) (weaken A (.shift .id)) :=
   by
     sorry
 
 theorem weakening_term : HasType Γ a A → IsType Γ B
-                         → HasType (Γ ⬝ B) (lift 0 1 a) (lift 0 1 A) :=
+                         → HasType (Γ ⬝ B) (weaken a (.shift .id)) 
+                           (weaken A (.shift .id)) :=
   by
     sorry
+
+theorem weakening_type_eq : IsEqualType Γ A A' → IsType Γ B
+                            → IsEqualType (Γ ⬝ B) (weaken A (.shift .id)) 
+                              (weaken A' (.shift .id)) :=
+  sorry
 
 -- FIXME: others like this?
-theorem weakening_type_eq : IsEqualType (Γ, Δ) A A' → IsType Γ B
-                            → IsEqualType (Γ ⬝ B, (lift_ctx 0 1 Δ))
-                              (lift (length_ctx Δ) 1 A) (lift (length_ctx Δ) 1 A') :=
-  by
-    sorry
+-- theorem weakening_type_eq : IsEqualType (concat_ctx Γ Δ) A A' → IsType Γ B
+--                             → IsEqualType (Γ ⬝ B, (lift_ctx 0 1 Δ))
+--                               (lift (length_ctx Δ) 1 A) (lift (length_ctx Δ) 1 A') :=
+--   by
+--     sorry
 
 theorem weakening_term_eq : IsEqualTerm Γ a a' A → IsType Γ B
-                            → IsEqualTerm (Γ ⬝ B) (lift 0 1 a) (lift 0 1 a') (lift 0 1 A') :=
+                            → IsEqualTerm (Γ ⬝ B) (weaken a (.shift .id)) 
+                              (weaken a' (.shift .id))
+                              (weaken A (.shift .id)) :=
   by
     sorry 
